Interop for Memcpy

src/test/interop/memcpy/Memcpy.fst
@@ -2,18 +2,82 @@ module Memcpy
 
 open FStar.Buffer
 open FStar.HyperStack.ST
+module HS = FStar.Monotonic.HyperStack
+
+open Vale_Sem
+open Machine_int
+open Interop
+module B = FStar.Buffer
 
 let bytes = buffer UInt8.t
 
-assume val memcpy_8: src:bytes -> dest:bytes ->
-  STL unit 
-  (requires (fun h -> live #UInt8.t h src /\ live #UInt8.t h dest /\ disjoint src dest 
-    /\ length #UInt8.t src == 1 /\ length #UInt8.t dest == 1))
-  (ensures  (fun h0 _ h1 -> live #UInt8.t h0 src /\ live #UInt8.t h0 dest /\ live #UInt8.t h1 dest /\ modifies_1 dest h0 h1
-    /\ length #UInt8.t src == 1 
-    /\ length #UInt8.t dest == 1
-    /\ (let d1 = as_seq #UInt8.t h1 dest in let d0 = as_seq #UInt8.t h0 dest in let s0 = as_seq #UInt8.t h0 src in
-  Seq.slice d1 0 1 ==
-	    Seq.slice s0 0 1
-	) ))
+let pre_cond (h:HS.mem) (src:bytes) (dest:bytes) =
+  live h src /\ live h dest /\ disjoint src dest /\ length src == 1 /\ length dest == 1
+
+let post_cond (h:HS.mem) (h':HS.mem) (src:bytes) (dest:bytes) =
+  live h src /\ live h dest /\ live h' src /\ live h' dest /\ disjoint src dest /\ length src == 1 /\ length dest == 1
+
+assume val memcpy: src:bytes -> dest:bytes ->
+  STL unit
+    (requires (fun h -> pre_cond h src dest))
+    (ensures (fun h0 _ h1 -> post_cond h0 h1 src dest))
+
+assume val src:bytes
+type doeq_src = b:bytes{disjoint_or_eq src b}
+
+assume val dst:doeq_src
+assume val addrs: addr_map
+type live_mem = m:HS.mem{live m src /\ live m dst}
+assume val mem:live_mem
+
+let buffers = [src; dst]
+assume val addr1:nat64
+assume val addr2:nat64
+
+let memcpy_code = Mov (OMem (MConst addr2)) (OMem (MConst addr1))
+
+let memcpy_vale (s:state) : state = eval_ins memcpy_code s
+
+let pre_v (s:state) = pre_cond (up_mem s.mem addrs buffers mem) src dst
+let post_v (s1:state) (s2:state) = post_cond (up_mem s1.mem addrs buffers mem)
+  (up_mem s2.mem addrs buffers mem) src dst
+
+let correct_memcpy (s:state) : Lemma
+  (requires (pre_v s))
+  (ensures (let s' = memcpy_vale s in post_v s s')) =
+  assume (addrs.[(as_addr src, idx src, length src)] == addr1);
+  assume (addrs.[(as_addr dst, idx dst, length dst)] == addr2);
+  let s' = memcpy_vale s in
+  let h0 = up_mem s.mem addrs buffers mem in
+  let h1 = up_mem s'.mem addrs buffers mem in
+  assume(live h1 src);
+  assume(live h1 dst);
+  ()
+
+#set-options "--z3rlimit 200"
+
+let correct_memcpy2 (s:state) : Lemma
+  (requires (pre_v s))
+  (ensures True) =
+  assume (addrs.[(as_addr src, idx src, length src)] == addr1);
+  assume (addrs.[(as_addr dst, idx dst, length dst)] == addr2);
+  let s' = memcpy_vale s in
+  let h0 = up_mem s.mem addrs buffers mem in
+  let h1 = up_mem s'.mem addrs buffers mem in
+  let d1 = as_seq h1 dst in
+  let d0 = as_seq h0 src in
+  // The property we actually want to prove
+  assert (Seq.equal d0 d1)
+
+// assume val memcpy_8: src:bytes -> dest:bytes ->
+//   STL unit 
+//   (requires (fun h -> live #UInt8.t h src /\ live #UInt8.t h dest /\ disjoint src dest 
+//     /\ length #UInt8.t src == 1 /\ length #UInt8.t dest == 1))
+//   (ensures  (fun h0 _ h1 -> live #UInt8.t h0 src /\ live #UInt8.t h0 dest /\ live #UInt8.t h1 dest /\ modifies_1 dest h0 h1
+//     /\ length #UInt8.t src == 1 
+//     /\ length #UInt8.t dest == 1
+//     /\ (let d1 = as_seq #UInt8.t h1 dest in let d0 = as_seq #UInt8.t h0 dest in let s0 = as_seq #UInt8.t h0 src in
+//   Seq.slice d1 0 1 ==
+// 	    Seq.slice s0 0 1
+// 	) ))
   
